read string

src/cbor/raw/pulse/everparse/CBOR.Pulse.Raw.Serialized.Base.fst
@@ -1,64 +1,13 @@
 module CBOR.Pulse.Raw.Serialized.Base
 friend CBOR.Pulse.Raw.Match.Serialized
 
+module Trade = Pulse.Lib.Trade.Util
+
 let dummy_initial_byte : initial_byte = { major_type = cbor_major_type_simple_value; additional_info = 0uy }
 
 let dummy_long_argument : long_argument dummy_initial_byte = LongArgumentOther dummy_initial_byte.additional_info () ()
 
 let dummy_header : header = (| dummy_initial_byte, dummy_long_argument |)
-
-```pulse
-ghost
-fn cbor_match_int_intro
-  (input: S.slice byte)
-  (pm: perm)
-  (v: raw_data_item)
-  (res: cbor_raw)
-  requires
-    pts_to_serialized serialize_raw_data_item input #pm v ** pure (CBOR_Case_Int? res)
-  ensures
-    trade (cbor_match 1.0R res v) (pts_to_serialized serialize_raw_data_item input #pm v)  
-{ 
-  ghost
-  fn aux (_: unit)
-     requires (pts_to_serialized serialize_raw_data_item input #pm v) ** cbor_match 1.0R res v
-     ensures pts_to_serialized serialize_raw_data_item input #pm v
-  {
-    unfold (cbor_match 1.0R (CBOR_Case_Int (CBOR_Case_Int?.v res)) v);
-    unfold (cbor_match_int (CBOR_Case_Int?.v res) v)
-  };
-  intro_trade _ _ _ aux
-}
-```
-
-```pulse
-fn cbor_match_string_intro
-  (input: S.slice byte)
-  (#pm: perm)
-  (#v: Seq.seq byte)
-  (c: cbor_string)
-  (r: raw_data_item)
-  requires
-    S.pts_to input #pm v ** pure (
-      input == c.cbor_string_ptr /\
-      pm == c.cbor_string_perm /\
-      Seq.length v == SZ.v (S.len c.cbor_string_ptr) /\
-      r == String c.cbor_string_type ({ size = c.cbor_string_size; value = U64.uint_to_t (SZ.v (S.len c.cbor_string_ptr)) }) v
-    )
-  ensures
-    cbor_match_string c 1.0R r **
-    trade (cbor_match_string c 1.0R r) (S.pts_to input #pm v)
-{
-  fold (cbor_match_string c 1.0R r);
-  ghost fn aux (_: unit)
-    requires emp ** cbor_match_string c 1.0R r
-    ensures S.pts_to input #pm v
-  {
-    unfold (cbor_match_string c 1.0R r)
-  };
-  intro_trade _ _ _ aux
-}
-```
 
 ```pulse
 fn cbor_read
@@ -83,23 +32,25 @@ fn cbor_read
     fold (cbor_match_int resi v);
     let res = CBOR_Case_Int resi;
     fold (cbor_match 1.0R res v);
-    cbor_match_int_intro input pm v res;
+    cbor_match_trade_int_intro (pts_to_serialized serialize_raw_data_item input #pm v) v res;
     res
   }
-(*
   else if (typ = cbor_major_type_text_string || typ = cbor_major_type_byte_string) {
     let i = get_string_length v h;
     get_string_payload pc v;
-    trade_trans _ _ (pts_to_serialized serialize_raw_data_item input #pm v);
+    Trade.trans _ _ (pts_to_serialized serialize_raw_data_item input #pm v);
     S.pts_to_len pc;
     with v' . assert (S.pts_to pc #pm v');
-    let res = CBOR_Case_String { cbor_string_type = typ; cbor_string_size = i.size; cbor_string_ptr = pc; cbor_string_perm = pm };
-    rewrite_with_trade
-      (S.pts_to pc #pm v')
+    let ress = { cbor_string_type = typ; cbor_string_size = i.size; cbor_string_ptr = pc; cbor_string_perm = pm };
+    cbor_match_string_intro pc ress v;
+    Trade.trans _ _ (pts_to_serialized serialize_raw_data_item input #pm v);
+    let res = CBOR_Case_String ress;
+    Trade.rewrite_with_trade
+      (cbor_match_string ress 1.0R v)
       (cbor_match 1.0R res v);
-    trade_trans _ _ (pts_to_serialized serialize_raw_data_item input #pm v);
+    Trade.trans _ _ (pts_to_serialized serialize_raw_data_item input #pm v);
+    res
   }
-*)
   else {
     admit ()
   }
